examples/n_german/nGerman.thy
@@ -1,0 +1,247 @@
+theory nGerman
+  imports CMP
+begin
+
+text \<open>Represents the three states: idle, shared, exclusive\<close>
+
+definition I :: scalrValueType where [simp]: "I \<equiv> enum ''control'' ''I''"
+definition S :: scalrValueType where [simp]: "S \<equiv> enum ''control'' ''S''"
+definition E :: scalrValueType where [simp]: "E \<equiv> enum ''control'' ''E''"
+
+text \<open>Control states\<close>
+
+definition Empty :: scalrValueType where [simp]: "Empty \<equiv> enum ''control'' ''Empty''"
+definition ReqS :: scalrValueType where [simp]: "ReqS \<equiv> enum ''control'' ''ReqS''"
+definition ReqE :: scalrValueType where [simp]: "ReqE \<equiv> enum ''control'' ''ReqE''"
+definition Inv :: scalrValueType where [simp]: "Inv \<equiv> enum ''control'' ''Inv''"
+definition InvAck :: scalrValueType where [simp]: "InvAck \<equiv> enum ''control'' ''InvAck''"
+definition GntS :: scalrValueType where [simp]: "GntS \<equiv> enum ''control'' ''GntS''"
+definition GntE ::scalrValueType where [simp]: "GntE \<equiv> enum ''control'' ''GntE''"
+
+definition true :: scalrValueType where [simp]: "true \<equiv> boolV True"
+definition false :: scalrValueType where [simp]: "false \<equiv> boolV False"
+
+definition n_RecvGntE :: "nat \<Rightarrow> rule" where
+  "n_RecvGntE i \<equiv>
+    let g = IVar (Para ''Chan2.Cmd'' i) =\<^sub>f Const GntE in
+    let a = assign (Para ''Cache.State'' i, Const E) ||
+            assign (Para ''Cache.Data'' i, IVar (Para ''Chan2.Data'' i)) ||
+            assign (Para ''Chan2.Cmd'' i, Const Empty) in
+      (guard g a)"
+
+lemma absRecvGntE:
+  "absTransfForm M (pre (n_RecvGntE i)) =
+    (IVar (Para ''Chan2.Cmd'' i) =\<^sub>f Const GntE)"
+  by (auto simp add: n_RecvGntE_def)
+
+definition n_RecvGntS :: "nat \<Rightarrow> rule" where
+  "n_RecvGntS i \<equiv>
+    let g = IVar (Para ''Chan2.Cmd'' i) =\<^sub>f Const GntS in
+    let a = assign (Para ''Cache.State'' i, Const S) ||
+            assign (Para ''Cache.Data'' i, IVar (Para ''Chan2.Data'' i)) ||
+            assign (Para ''Chan2.Cmd'' i, Const Empty) in
+      (guard g a)"
+
+lemma absRecvGntS:
+  "absTransfForm M (pre (n_RecvGntS i)) =
+    (IVar (Para ''Chan2.Cmd'' i) =\<^sub>f Const GntS)"
+  by (auto simp add: n_RecvGntS_def)
+
+definition n_SendGntE:: "nat \<Rightarrow> nat \<Rightarrow> rule" where
+  "n_SendGntE N i \<equiv>
+    let g = IVar (Ident ''CurCmd'') =\<^sub>f Const ReqE \<and>\<^sub>f
+            IVar (Ident ''CurPtr'') =\<^sub>f Const (index i) \<and>\<^sub>f
+            IVar (Para ''Chan2.Cmd'' i) =\<^sub>f Const Empty \<and>\<^sub>f
+            IVar (Ident ''ExGntd'') =\<^sub>f Const false \<and>\<^sub>f
+            (\<forall>\<^sub>fj. IVar (Para ''ShrSet'' j) =\<^sub>f Const false) N in
+    let a = assign (Para ''Chan2.Cmd'' i, Const GntE) ||
+            assign (Para ''Chan2.Data'' i, IVar (Ident ''MemData'')) ||
+            assign (Para ''ShrSet'' i, Const true) ||
+            assign (Ident ''ExGntd'', Const true) ||
+            assign (Ident ''CurCmd'', Const Empty) in
+      (guard g a)"
+
+lemma absSendGntE:
+  "absTransfForm M (pre (n_SendGntE N i)) =
+    undefined"
+  unfolding n_SendGntE_def Let_def pre.simps
+  apply auto
+  sorry
+
+definition n_SendGntS :: "nat \<Rightarrow> rule" where
+  "n_SendGntS i \<equiv>
+    let g = IVar (Ident ''CurCmd'') =\<^sub>f Const ReqS \<and>\<^sub>f
+            IVar (Ident ''CurPtr'') =\<^sub>f Const (index i) \<and>\<^sub>f
+            IVar (Para ''Chan2.Cmd'' i) =\<^sub>f Const Empty \<and>\<^sub>f
+            IVar (Ident ''ExGntd'') =\<^sub>f Const false in
+    let a = assign (Para ''Chan2.Cmd'' i, Const GntS) ||
+            assign (Para ''Chan2.Data'' i, IVar (Ident ''MemData'')) ||
+            assign (Para ''ShrSet'' i, Const true) ||
+            assign (Ident ''CurCmd'', Const Empty) in
+      (guard g a)"
+
+definition n_RecvInvAck1 :: "nat \<Rightarrow> rule" where
+  "n_RecvInvAck1 i \<equiv>
+    let g = IVar (Para ''Chan3.Cmd'' i) =\<^sub>f Const InvAck \<and>\<^sub>f
+            \<not>\<^sub>f IVar (Ident ''CurCmd'') =\<^sub>f Const Empty \<and>\<^sub>f
+            IVar (Ident ''ExGntd'') =\<^sub>f Const true in
+    let a = assign (Para ''Chan3.Cmd'' i, Const Empty) ||
+            assign (Para ''ShrSet'' i, Const false) ||
+            assign (Ident ''ExGntd'', Const false) ||
+            assign (Ident ''MemData'', IVar (Para ''Chan3.Data'' i)) in
+      (guard g a)"
+
+definition n_RecvInvAck2 :: "nat \<Rightarrow> rule" where
+  "n_RecvInvAck2 i \<equiv>
+    let g = IVar (Para ''Chan3.Cmd'' i) =\<^sub>f Const InvAck \<and>\<^sub>f
+            \<not>\<^sub>f IVar (Ident ''CurCmd'') =\<^sub>f Const Empty \<and>\<^sub>f
+            \<not>\<^sub>f IVar (Ident ''ExGntd'') =\<^sub>f Const true in
+    let a = assign (Para ''Chan3.Cmd'' i, Const Empty) ||
+            assign (Para ''ShrSet'' i, Const false) in
+      (guard g a)"
+
+definition n_SendInvAck1 :: "nat \<Rightarrow> rule" where
+  "n_SendInvAck1 i \<equiv>
+    let g = IVar (Para ''Chan2.Cmd'' i) =\<^sub>f Const Inv \<and>\<^sub>f
+            IVar (Para ''Chan3.Cmd'' i) =\<^sub>f Const Empty \<and>\<^sub>f
+            IVar (Para ''Cache.State'' i) =\<^sub>f Const E in
+    let a = assign (Para ''Chan2.Cmd'' i, Const Empty) ||
+            assign (Para ''Chan3.Cmd'' i, Const InvAck) ||
+            assign (Para ''Chan3.Data'' i, IVar (Para ''Cache.Data'' i)) ||
+            assign (Para ''Cache.State'' i, Const I) in
+      (guard g a)"
+
+definition n_SendInvAck2 :: "nat \<Rightarrow> rule" where
+  "n_SendInvAck2 i \<equiv>
+    let g = IVar (Para ''Chan2.Cmd'' i) =\<^sub>f Const Inv \<and>\<^sub>f
+            IVar (Para ''Chan3.Cmd'' i) =\<^sub>f Const Empty \<and>\<^sub>f
+            \<not>\<^sub>f IVar (Para ''Cache.State'' i) =\<^sub>f Const E in
+    let a = assign (Para ''Chan2.Cmd'' i, Const Empty) ||
+            assign (Para ''Chan3.Cmd'' i, Const InvAck) ||
+            assign (Para ''Cache.State'' i, Const I) in
+      (guard g a)"
+
+definition n_SendInv1 :: "nat \<Rightarrow> rule" where
+  "n_SendInv1 i \<equiv>
+    let g = IVar (Para ''Chan2.Cmd'' i) =\<^sub>f Const Empty \<and>\<^sub>f
+            IVar (Para ''InvSet'' i) =\<^sub>f Const true \<and>\<^sub>f
+            IVar (Ident ''CurCmd'') =\<^sub>f Const ReqE in
+    let a = assign (Para ''Chan2.Cmd'' i, Const Inv) ||
+            assign (Para ''InvSet'' i, Const false) in
+      (guard g a)"
+
+definition n_SendInv2 :: "nat \<Rightarrow> rule" where
+  "n_SendInv2 i \<equiv>
+    let g = IVar (Para ''Chan2.Cmd'' i) =\<^sub>f Const Empty \<and>\<^sub>f
+            IVar (Para ''InvSet'' i) =\<^sub>f Const true \<and>\<^sub>f
+            IVar (Ident ''CurCmd'') =\<^sub>f Const ReqS \<and>\<^sub>f
+            IVar (Ident ''ExGntd'') =\<^sub>f Const true in
+    let a = assign (Para ''Chan2.Cmd'' i, Const Inv) ||
+            assign (Para ''InvSet'' i, Const false) in
+      (guard g a)"
+
+definition n_RecvReqE :: "nat \<Rightarrow> nat \<Rightarrow> rule" where
+  "n_RecvReqE N i \<equiv>
+    let g = IVar (Ident ''CurCmd'') =\<^sub>f Const Empty \<and>\<^sub>f
+            IVar (Para ''Chan1.Cmd'' i) =\<^sub>f Const ReqE in
+    let a = assign (Ident ''CurCmd'', Const ReqE) ||
+            assign (Ident ''CurPtr'', Const (index i)) ||
+            assign (Para ''Chan1.Cmd'' i, Const Empty) ||
+            forallStm (\<lambda>j. assign (Para ''InvSet'' j, IVar (Para ''ShrSet'' j))) N in
+      (guard g a)"
+
+definition n_RecvReqS :: "nat \<Rightarrow> nat \<Rightarrow> rule" where
+  "n_RecvReqS N i \<equiv>
+    let g = IVar (Ident ''CurCmd'') =\<^sub>f Const Empty \<and>\<^sub>f
+            IVar (Para ''Chan1.Cmd'' i) =\<^sub>f Const ReqS in
+    let a = assign (Ident ''CurCmd'', Const ReqS) ||
+            assign (Ident ''CurPtr'', Const (index i)) ||
+            assign (Para ''Chan1.Cmd'' i, Const Empty) ||
+            forallStm (\<lambda>j. assign (Para ''InvSet'' j, IVar (Para ''ShrSet'' j))) N in
+      (guard g a)"
+
+definition n_SendReqE1 :: "nat \<Rightarrow> rule" where
+  "n_SendReqE1 i \<equiv>
+    let g = IVar (Para ''Chan1.Cmd'' i) =\<^sub>f Const Empty \<and>\<^sub>f
+            IVar (Para ''Cache.State'' i) =\<^sub>f Const I in
+    let a = assign (Para ''Chan1.Cmd'' i, Const ReqE) in
+      (guard g a)"
+
+definition n_SendReqE2 :: "nat \<Rightarrow> rule" where
+  "n_SendReqE2 i \<equiv>
+    let g = IVar (Para ''Chan1.Cmd'' i) =\<^sub>f Const Empty \<and>\<^sub>f
+            IVar (Para ''Cache.State'' i) =\<^sub>f Const S in
+    let a = assign (Para ''Chan1.Cmd'' i, Const ReqE) in
+      (guard g a)"
+
+definition n_SendReqS :: "nat \<Rightarrow> rule" where
+  "n_SendReqS i \<equiv>
+    let g = IVar (Para ''Chan1.Cmd'' i) =\<^sub>f Const Empty \<and>\<^sub>f
+            IVar (Para ''Cache.State'' i) =\<^sub>f Const I in
+    let a = assign (Para ''Chan1.Cmd'' i, Const ReqS) in
+      (guard g a)"
+
+definition n_Store :: "nat \<Rightarrow> rule" where
+  "n_Store i \<equiv>
+    let g = IVar (Para ''Cache.State'' i) =\<^sub>f Const E in
+    let a = assign (Para ''Cache.Data'' i, IVar (Ident ''d'')) ||
+            assign (Ident ''AuxData'', IVar (Ident ''d'')) in
+      (guard g a)"
+
+definition rules::"nat \<Rightarrow> rule set" where
+  "rules N \<equiv> {r.
+    (\<exists>i. i\<le>N \<and> r=n_RecvGntE i) \<or>
+    (\<exists>i. i\<le>N \<and> r=n_RecvGntS i) \<or>
+    (\<exists>i. i\<le>N \<and> r=n_SendGntE N i) \<or>
+    (\<exists>i. i\<le>N \<and> r=n_SendGntS i) \<or>
+    (\<exists>i. i\<le>N \<and> r=n_RecvInvAck1 i) \<or>
+    (\<exists>i. i\<le>N \<and> r=n_RecvInvAck2 i) \<or>
+    (\<exists>i. i\<le>N \<and> r=n_SendInvAck1 i) \<or>
+    (\<exists>i. i\<le>N \<and> r=n_SendInvAck2 i) \<or>
+    (\<exists>i. i\<le>N \<and> r=n_SendInv1 i) \<or>
+    (\<exists>i. i\<le>N \<and> r=n_SendInv2 i) \<or>
+    (\<exists>i. i\<le>N \<and> r=n_RecvReqE N i) \<or>
+    (\<exists>i. i\<le>N \<and> r=n_RecvReqS N i) \<or>
+    (\<exists>i. i\<le>N \<and> r=n_SendReqE1 i) \<or>
+    (\<exists>i. i\<le>N \<and> r=n_SendReqE2 i) \<or>
+    (\<exists>i. i\<le>N \<and> r=n_SendReqS i) \<or>
+    (\<exists>i. i\<le>N \<and> r=n_Store i)
+  }"
+
+definition initSpec0 :: "nat \<Rightarrow> formula" where
+  "initSpec0 N \<equiv> (\<forall>\<^sub>fi. IVar (Para ''Chan1.Cmd'' i) =\<^sub>f Const Empty) N"
+
+definition initSpec1 :: "nat \<Rightarrow> formula" where
+  "initSpec1 N \<equiv> (\<forall>\<^sub>fi. IVar (Para ''Chan2.Cmd'' i) =\<^sub>f Const Empty) N"
+
+definition initSpec2 :: "nat \<Rightarrow> formula" where
+  "initSpec2 N \<equiv> (\<forall>\<^sub>fi. IVar (Para ''Chan3.Cmd'' i) =\<^sub>f Const Empty) N"
+
+definition initSpec3 :: "nat \<Rightarrow> formula" where
+  "initSpec3 N \<equiv> (\<forall>\<^sub>fi. IVar (Para ''Cache.State'' i) =\<^sub>f Const I) N"
+
+definition initSpec4 :: "nat \<Rightarrow> formula" where
+  "initSpec4 N \<equiv> (\<forall>\<^sub>fi. IVar (Para ''InvSet'' i) =\<^sub>f Const false) N"
+
+definition initSpec5 :: "nat \<Rightarrow> formula" where
+  "initSpec5 N \<equiv> (\<forall>\<^sub>fi. IVar (Para ''ShrSet'' i) =\<^sub>f Const false) N"
+
+definition initSpec6 :: formula where
+  "initSpec6 \<equiv> IVar (Ident ''ExGntd'') =\<^sub>f Const false"
+
+definition initSpec7 :: formula where
+  "initSpec7 \<equiv> IVar (Ident ''CurCmd'') =\<^sub>f Const Empty"
+
+definition allInitSpecs :: "nat \<Rightarrow> formula list" where
+  "allInitSpecs N \<equiv> [
+    (initSpec0 N),
+    (initSpec1 N),
+    (initSpec2 N),
+    (initSpec3 N),
+    (initSpec4 N),
+    (initSpec5 N),
+    initSpec6,
+    initSpec7
+  ]"
+
+end
